ShaFv.lean
@@ -1,1 +1,2 @@
+import ShaFv.RISCV.Machine
 import ShaFv.SHA3.Root
