lakefile.lean
@@ -4,7 +4,11 @@ open Lake DSL
 package sha_fv_experiment where
 
 require «cryptography» from "./specs/sha-3"
-require repl from git "https://github.com/leanprover-community/repl.git" @ "v4.27.0"
+require repl from git "https://github.com/leanprover-community/repl.git" @ "v4.26.0"
+
+lean_lib LeanRV64DExecutable where
+  srcDir := "build/sail-riscv-lean"
+  moreLeanArgs := #["--tstack=400000"]
 
 @[default_target]
 lean_lib ShaFv where
